TabularTypeInterpreter/F⊗⊕ω/Lemmas/Kind.lean
@@ -1,0 +1,9 @@
+import TabularTypeInterpreter.«F⊗⊕ω».Syntax.Kind
+
+namespace TabularTypeInterpreter.«F⊗⊕ω»
+
+@[simp]
+theorem Kind.sizeOf_pos (K : Kind) : 0 < sizeOf K := by
+  induction K <;> simp_arith
+
+end TabularTypeInterpreter.«F⊗⊕ω»
